src/Manifest.v
@@ -86,7 +86,7 @@ Definition empty_PolicyT : PolicyT := [].
     my_abstract_plc   : Plc ; 
 
     asps              : manifest_set ASP_ID; 
-    appraisal_asps    : manifest_set (Plc * ASP_ID) ;
+    appraisal_asps    : manifest_set ASP_ID ;
     uuidPlcs          : manifest_set Plc ;
     pubKeyPlcs        : manifest_set Plc ;
     targetPlcs        : manifest_set Plc ;
@@ -111,8 +111,11 @@ Definition empty_PolicyT : PolicyT := [].
     UUID_AM_Clone : UUID ;
 
     (* Local Mappings *)
+    Lib_ASPs            : MapC ASP_ID Concrete_ASP_ID ;
     Lib_Plcs            : MapC Plc UUID ;
     Lib_PubKeys         : MapC Plc PublicKey ;
+    (* Attest <-> Appraisal ASP Mapping *)
+    ASP_Compat_Map      : MapC ASP_ID ASP_ID ;
   }.
 
 Record AM_Config : Type := 
@@ -120,7 +123,6 @@ Record AM_Config : Type :=
     absMan : Manifest ;
     am_clone_addr : UUID ;
     aspCb : (ASPCallback DispatcherErrors) ;
-    app_aspCb : (ASPCallback DispatcherErrors) ;
     plcCb : PlcCallback ;
     pubKeyCb : PubKeyCallback ;
   }.
@@ -133,7 +135,6 @@ Definition empty_aspCb (ps:ASP_PARAMS) (rawev:RawEv)
   mkAmConfig 
     empty_Manifest
     default_uuid
-    empty_aspCb
     empty_aspCb
     (fun x => errC Unavailable)
     (fun x => errC Unavailable).
