src/Manifest_JSON.v
@@ -4,7 +4,7 @@ Import ListNotations ResultNotation.
 
 
 Definition Manifest_to_JSON (m : Manifest) : JSON :=
-  let '(Build_Manifest my_abstract_plc asps appraisal_asps uuidPlcs pubKeyPlcs targetPlcs policy) := m 
+  let '(Build_Manifest my_abstract_plc asps appr_asps uuidPlcs pubKeyPlcs targetPlcs policy) := m 
   in
     JSON_Object [
       (MAN_ABS_PLC, 
@@ -12,7 +12,7 @@ Definition Manifest_to_JSON (m : Manifest) : JSON :=
       (MAN_ASPS, 
         (InJSON_Array (manifest_set_to_list_InJson asps)));
       (MAN_APPR_ASPS, 
-        (InJSON_Array (manifest_set_pairs_to_list_InJson appraisal_asps)));
+        (InJSON_Array (manifest_set_to_list_InJson appr_asps)));
       (MAN_UUID_PLCS, 
         (InJSON_Array (manifest_set_to_list_InJson uuidPlcs)));
       (MAN_PUBKEY_PLCS, 
@@ -34,7 +34,7 @@ Definition JSON_to_Manifest (js : JSON) : ResultT Manifest string :=
 
   ABS_PLC <- from_string temp_ABS_PLC;;
   ASPS <- list_InJson_to_manifest_set temp_ASPS;;
-  APPR_ASPS <- list_InJson_to_manifest_set_pairs temp_APPR_ASPS;;
+  APPR_ASPS <- list_InJson_to_manifest_set temp_APPR_ASPS;;
   UUID_PLCS <- list_InJson_to_manifest_set temp_UUID_PLCS;;
   PUBKEY_PLCS <- list_InJson_to_manifest_set temp_PUBKEY_PLCS;;
   TARGET_PLCS <- list_InJson_to_manifest_set temp_TARGET_PLCS;;
@@ -54,23 +54,29 @@ try congruence; repeat find_injection; eauto.
 Defined.
 
 Definition AM_Lib_to_JSON (am : AM_Library) : JSON :=
-  let '(Build_AM_Library clone_uuid lib_plcs lib_pubkeys) := am
+  let '(Build_AM_Library clone_uuid lib_asps lib_plcs lib_pubkeys compat_asps_map) := am
   in
     JSON_Object [
       (AM_CLONE_UUID, (InJSON_String (to_string clone_uuid)));
+      (AM_LIB_ASPS, (InJSON_Object (to_JSON lib_asps)));
       (AM_LIB_PLCS, (InJSON_Object (to_JSON lib_plcs)));
-      (AM_LIB_PUBKEYS, (InJSON_Object (to_JSON lib_pubkeys)))
+      (AM_LIB_PUBKEYS, (InJSON_Object (to_JSON lib_pubkeys)));
+      (AM_LIB_COMPAT_ASPS, (InJSON_Object (to_JSON compat_asps_map)))
     ].
 
 Definition JSON_to_AM_Lib (js : JSON) : ResultT AM_Library string :=
   temp_CLONE_UUID <- JSON_get_string AM_CLONE_UUID js;;
+  temp_LIB_ASPS <- JSON_get_Object AM_LIB_ASPS js;;
   temp_LIB_PLCS <- JSON_get_Object AM_LIB_PLCS js;;
   temp_LIB_PUBKEYS <- JSON_get_Object AM_LIB_PUBKEYS js;;
+  temp_COMPAT_ASPS <- JSON_get_Object AM_LIB_COMPAT_ASPS js;;
 
   CLONE_UUID <- from_string temp_CLONE_UUID;;
+  LIB_ASPS <- from_JSON temp_LIB_ASPS;;
   LIB_PLCS <- from_JSON temp_LIB_PLCS;;
   LIB_PUBKEYS <- from_JSON temp_LIB_PUBKEYS;;
-  resultC (Build_AM_Library CLONE_UUID LIB_PLCS LIB_PUBKEYS).
+  COMPAT_ASPS <- from_JSON temp_COMPAT_ASPS;;
+  resultC (Build_AM_Library CLONE_UUID LIB_ASPS LIB_PLCS LIB_PUBKEYS COMPAT_ASPS).
 
 Global Instance Jsonifiable_AM_Library : Jsonifiable AM_Library.
 eapply Build_Jsonifiable with
@@ -80,7 +86,7 @@ intuition; destruct a; simpl in *.
 unfold JSON_to_AM_Lib, res_bind; simpl in *;
 repeat rewrite canonical_stringification in *;
 repeat (try break_match; simpl in *; subst; try find_injection; try find_rewrite; eauto; try congruence);
-repeat match goal with
+try (repeat match goal with
 | H : result_map _ (map _ ?l) = errC _ |- _ => 
     induction l; simpl in *; intuition; try congruence;
     unfold res_bind in *; repeat (try break_match; simpl in *; subst; intuition; eauto; try find_injection; try find_rewrite; try congruence);
@@ -94,5 +100,5 @@ repeat match goal with
       repeat rewrite canonical_stringification in *; try congruence;
       repeat find_injection; eauto;
       erewrite IH'; eauto); subst; clear H; eauto
-end.
+end; fail).
 Defined.
